refactored

thy/Semantics_Ternary/Primitive_Normalization.thy
@@ -566,4 +566,187 @@ lemma not_has_disc_normalize_match: "\<not> has_disc_negated disc neg  m \<longr
 
 
 
+
+
+subsection{*Optimizing a match expression*}
+
+  text{*Optimizes a match expression with a function that takes @{typ "'b negation_type list"}
+  and returns @{typ "('b list \<times> 'b list) option"}.
+  The function should return @{const None} if the match expression cannot match.
+  It returns @{term "Some (as_pos, as_neg)"} where @{term as_pos} and @{term as_neg} are lists of
+  primitives. Positive and Negated.
+  The result is one match expression.
+
+  In contrast @{const normalize_primitive_extract} returns a list of match expression, to be read es their disjunction.*}
+
+  definition compress_normalize_primitive :: "(('a \<Rightarrow> bool) \<times> ('a \<Rightarrow> 'b)) \<Rightarrow> ('b \<Rightarrow> 'a) \<Rightarrow>
+                                              ('b negation_type list \<Rightarrow> ('b list \<times> 'b list) option) \<Rightarrow> 
+                                              'a match_expr \<Rightarrow> 'a match_expr option" where 
+    "compress_normalize_primitive disc_sel C f m \<equiv> (case primitive_extractor disc_sel m of (as, rst) \<Rightarrow>
+      (map_option (\<lambda>(as_pos, as_neg). MatchAnd
+                                       (alist_and (NegPos_map C ((map Pos as_pos)@(map Neg as_neg))))
+                                       rst
+                  ) (f as)))"
+
+
+
+  lemma compress_normalize_primitive_nnf: "wf_disc_sel disc_sel C \<Longrightarrow> 
+      normalized_nnf_match m \<Longrightarrow> compress_normalize_primitive disc_sel C f m = Some m' \<Longrightarrow>
+    normalized_nnf_match m'"
+    apply(case_tac "primitive_extractor disc_sel m")
+    apply(simp add: compress_normalize_primitive_def)
+    apply(clarify)
+    apply (simp add: normalized_nnf_match_alist_and)
+    apply(cases disc_sel, simp)
+    using primitive_extractor_correct(2) by blast
+
+
+  lemma compress_normalize_primitive_not_introduces_C:
+    assumes notdisc: "\<not> has_disc disc m"
+        and wf: "wf_disc_sel (disc,sel) C"
+        and nm: "normalized_nnf_match m"
+        and some: "compress_normalize_primitive (disc,sel) C f m = Some m'"
+        and f_preserves: "\<And>as_pos as_neg. f [] = Some (as_pos, as_neg) \<Longrightarrow> as_pos = [] \<and> as_neg = []"
+     shows "\<not> has_disc disc m'"
+   proof -
+        obtain as ms where asms: "primitive_extractor (disc, sel) m = (as, ms)" by fastforce
+        from notdisc primitive_extractor_correct(4)[OF nm wf asms] have 1: "\<not> has_disc disc ms" by simp
+        from notdisc primitive_extractor_correct(7)[OF nm wf asms] have 2: "as = [] \<and> ms = m" by simp
+        from 1 2 some show ?thesis by(auto dest: f_preserves simp add: compress_normalize_primitive_def asms)
+   qed
+
+  lemma compress_normalize_primitive_not_introduces_C_negated:
+    assumes notdisc: "\<not> has_disc_negated disc False m"
+        and wf: "wf_disc_sel (disc,sel) C"
+        and nm: "normalized_nnf_match m"
+        and some: "compress_normalize_primitive (disc,sel) C f m = Some m'"
+        and f_preserves: "\<And>as as_pos as_neg. f as = Some (as_pos, as_neg) \<Longrightarrow> getNeg as = [] \<Longrightarrow> as_neg = []"
+     shows "\<not> has_disc_negated disc False m'"
+   proof -
+        obtain as ms where asms: "primitive_extractor (disc,sel) m = (as, ms)" by fastforce
+        from notdisc primitive_extractor_correct(6)[OF nm wf asms] have 1: "\<not> has_disc_negated disc False ms" by simp
+        from asms notdisc has_disc_negated_primitive_extractor[OF nm, where disc=disc and sel=sel] have
+          "\<forall>a. Neg a \<notin> set as" by(simp)
+        hence "getNeg as = []" by (meson NegPos_set(5) image_subset_iff last_in_set)
+        with f_preserves have f_preserves': "\<And>as_pos as_neg. f as = Some (as_pos, as_neg) \<Longrightarrow> as_neg = []" by simp
+        from 1 have "\<And> a b.\<not> has_disc_negated disc False (MatchAnd (alist_and (NegPos_map C (map Pos a))) ms)"
+          by(simp add: has_disc_negated_alist_and NegPos_map_map_Pos negation_type_to_match_expr_simps)
+        with some show ?thesis by(auto dest: f_preserves' simp add: compress_normalize_primitive_def asms)
+   qed
+
+
+
+
+  lemma compress_normalize_primitive_Some:
+  assumes normalized: "normalized_nnf_match m"
+      and wf: "wf_disc_sel (disc,sel) C"
+      and some: "compress_normalize_primitive (disc,sel) C f m = Some m'"
+      and f_correct: "\<And>as as_pos as_neg. f as = Some (as_pos, as_neg) \<Longrightarrow>
+            matches \<gamma> (alist_and (NegPos_map C ((map Pos as_pos)@(map Neg as_neg)))) a p \<longleftrightarrow>
+            matches \<gamma> (alist_and (NegPos_map C as)) a p"
+    shows "matches \<gamma> m' a p \<longleftrightarrow> matches \<gamma> m a p"
+    using some
+    apply(simp add: compress_normalize_primitive_def)
+    apply(case_tac "primitive_extractor (disc,sel) m")
+    apply(rename_tac as rst, simp)
+    apply(drule primitive_extractor_correct(1)[OF normalized wf, where \<gamma>=\<gamma> and a=a and p=p])
+    apply(elim exE conjE)
+    apply(drule f_correct)
+    by (meson alist_and_append bunch_of_lemmata_about_matches(1))
+    
+
+  lemma compress_normalize_primitive_None:
+  assumes normalized: "normalized_nnf_match m"
+      and wf: "wf_disc_sel (disc,sel) C"
+      and none: "compress_normalize_primitive (disc,sel) C f m = None"
+      and f_correct: "\<And>as. f as = None \<Longrightarrow> \<not> matches \<gamma> (alist_and (NegPos_map C as)) a p"
+    shows "\<not> matches \<gamma> m a p"
+    using none
+    apply(simp add: compress_normalize_primitive_def)
+    apply(case_tac "primitive_extractor (disc, sel) m")
+    apply(auto dest: primitive_extractor_correct(1)[OF assms(1) wf] f_correct)
+    done
+
+
+
+  (* only for arbitrary discs that do not match C*)
+  lemma compress_normalize_primitive_hasdisc:
+    assumes am: "\<not> has_disc disc2 m"
+        and wf: "wf_disc_sel (disc,sel) C"
+        and disc: "(\<forall>a. \<not> disc2 (C a))"
+        and nm: "normalized_nnf_match m"
+        and some: "compress_normalize_primitive (disc,sel) C f m = Some m'"
+     shows "normalized_nnf_match m' \<and> \<not> has_disc disc2 m'"
+   proof -
+        from compress_normalize_primitive_nnf[OF wf nm some] have goal1: "normalized_nnf_match m'" .
+        obtain as ms where asms: "primitive_extractor (disc, sel) m = (as, ms)" by fastforce
+        from am primitive_extractor_correct(4)[OF nm wf asms] have 1: "\<not> has_disc disc2 ms" by simp
+        { fix is_pos is_neg
+          from disc have x1: "\<not> has_disc disc2 (alist_and (NegPos_map C (map Pos is_pos)))"
+            by(simp add: has_disc_alist_and NegPos_map_map_Pos negation_type_to_match_expr_simps)
+          from disc have x2: "\<not> has_disc disc2 (alist_and (NegPos_map C (map Neg is_neg)))"
+            by(simp add: has_disc_alist_and NegPos_map_map_Neg negation_type_to_match_expr_simps)
+          from x1 x2 have "\<not> has_disc disc2 (alist_and (NegPos_map C (map Pos is_pos @ map Neg is_neg)))"
+            apply(simp add: NegPos_map_append has_disc_alist_and) by blast
+        }
+        with some have "\<not> has_disc disc2 m'"
+          apply(simp add: compress_normalize_primitive_def asms)
+          apply(elim exE conjE)
+          using 1 by force
+        with goal1 show ?thesis by simp
+   qed
+  lemma compress_normalize_primitive_hasdisc_negated:
+    assumes am: "\<not> has_disc_negated disc2 neg m"
+        and wf: "wf_disc_sel (disc,sel) C"
+        and disc: "(\<forall>a. \<not> disc2 (C a))"
+        and nm: "normalized_nnf_match m"
+        and some: "compress_normalize_primitive (disc,sel) C f m = Some m'"
+     shows "normalized_nnf_match m' \<and> \<not> has_disc_negated disc2 neg m'"
+   proof -
+        from compress_normalize_primitive_nnf[OF wf nm some] have goal1: "normalized_nnf_match m'" .
+        obtain as ms where asms: "primitive_extractor (disc, sel) m = (as, ms)" by fastforce
+        from am primitive_extractor_correct(6)[OF nm wf asms] have 1: "\<not> has_disc_negated disc2 neg ms" by simp
+        { fix is_pos is_neg
+          from disc have x1: "\<not> has_disc_negated disc2 neg (alist_and (NegPos_map C (map Pos is_pos)))"
+            by(simp add: has_disc_negated_alist_and NegPos_map_map_Pos negation_type_to_match_expr_simps)
+          from disc have x2: "\<not> has_disc_negated disc2 neg (alist_and (NegPos_map C (map Neg is_neg)))"
+            by(simp add: has_disc_negated_alist_and NegPos_map_map_Neg negation_type_to_match_expr_simps)
+          from x1 x2 have "\<not> has_disc_negated disc2 neg (alist_and (NegPos_map C (map Pos is_pos @ map Neg is_neg)))"
+            apply(simp add: NegPos_map_append has_disc_negated_alist_and) by blast
+        }
+        with some have "\<not> has_disc_negated disc2 neg m'"
+          apply(simp add: compress_normalize_primitive_def asms)
+          apply(elim exE conjE)
+          using 1 by force
+        with goal1 show ?thesis by simp
+   qed
+
+
+  thm normalize_primitive_extract_preserves_unrelated_normalized_n_primitive (*is similar*)
+  lemma compress_normalize_primitve_preserves_normalized_n_primitive:
+    assumes am: "normalized_n_primitive (disc2, sel2) P m"
+        and wf: "wf_disc_sel (disc,sel) C"
+        and disc: "(\<forall>a. \<not> disc2 (C a))"
+        and nm: "normalized_nnf_match m"
+        and some: "compress_normalize_primitive (disc,sel) C f m = Some m'"
+     shows "normalized_nnf_match m' \<and> normalized_n_primitive (disc2, sel2) P m'"
+   proof -
+        from compress_normalize_primitive_nnf[OF wf nm some] have goal1: "normalized_nnf_match m'" .
+        obtain as ms where asms: "primitive_extractor (disc, sel) m = (as, ms)" by fastforce
+        from am primitive_extractor_correct[OF nm wf asms] have 1: "normalized_n_primitive (disc2, sel2) P ms" by fast
+        { fix iss
+          from disc have "normalized_n_primitive (disc2, sel2) P (alist_and (NegPos_map C iss))"
+            apply(induction iss)
+             apply(simp_all)
+            apply(rename_tac i iss, case_tac i)
+             apply(simp_all)
+            done
+        }
+        with some have "normalized_n_primitive (disc2, sel2) P m'"
+          apply(simp add: compress_normalize_primitive_def asms)
+          apply(elim exE conjE)
+          using 1 by force
+        with goal1 show ?thesis by simp
+   qed
+  
 end
